platform/cito/HeapFacts.v
@@ -1,0 +1,5 @@
+Require Import Semantics.
+
+Lemma heap_merge_empty : forall h, heap_merge h heap_empty = h.
+  admit.
+Qed.
