platform/cito/Layout.v
@@ -1,0 +1,8 @@
+Require Import AutoSep.
+Require Import Semantics.
+
+Set Implicit Arguments.
+
+Definition Layout := W -> ADTValue -> HProp.
+
+Variable layout : Layout.
