platform/cito/LayoutHints2.v
@@ -1,0 +1,15 @@
+Require Import Inv.
+Require Import Semantics.
+
+Set Implicit Arguments.
+
+Definition heap_to_split h (_ : list (W * ArgIn)) := is_heap h.
+
+Lemma split_heap : forall h pairs, good_inputs h pairs -> heap_to_split h pairs ===> let h1 := make_heap pairs in is_heap h1 * is_heap (heap_diff h h1).
+  admit.
+Qed.
+
+Definition hints_split_heap : TacPackage.
+  prepare split_heap tt.
+Defined.
+
