platform/cito/SepLemmas.v
@@ -1,16 +1,3 @@
-Require Import Inv.
-Require Import Semantics.
-
-Set Implicit Arguments.
-
-Lemma is_heap_upd_option_bwd : forall layout h addr a, is_heap layout h * layout_option layout addr a ===> is_heap layout (heap_upd_option h addr a).
-  admit.
-Qed.
-
-Lemma star_separated : forall layout specs st other h addr adt, interp specs (![is_heap layout h * layout_option layout addr adt * other] st) -> separated h addr adt.
-  admit.
-Qed.
-
 (*
 Lemma star_diff_ptrs : forall specs st p1 p2, interp specs (![p1 =?>1 * p2 =?> 1] st) -> p1 <> p2.
   rewrite sepFormula_eq.
